update program evm

src/instr.v
@@ -159,7 +159,9 @@ Inductive Instr :=
 | BADINSTR.
 
     
-(* From nat to Instr *)
+(*-------------------------------------------------------------------
+ From nat to Instr
+ -------------------------------------------------------------------*)
 Definition fromNatToInstr (n : nat) : Instr :=
   match n with
     | 0 => STOP
@@ -305,6 +307,160 @@ Definition fromNatToInstr (n : nat) : Instr :=
     | _ => BADINSTR
   end.
 
+(*--------------------------------------------------------------------
+ Instr to string for assembly decoder.
+ --------------------------------------------------------------------*)
+From Coq Require Import ZArith.ZArith Strings.String.
+Import Ascii.
 
-(* Unit test *)
+Definition instrToString (i : Instr) :=
+  (match i with
+          (* Stop and arithmetic operations *)
+| STOP => "STOP"
+| ADD => "ADD"
+| MUL => "MUL"
+| SUB => "SUB"
+| DIV => "DIV"
+| SDIV => "SDIV"
+| MOD => "MOD"
+| SMOD => "SMOD"
+| ADDMOD => "ADDMOD"
+| MULMOD => "MULMOD"
+| EXP => "EXP"
+| SIGNEXTEND => "SIGNEXTEND"
+    (* Comparison and bitwise logic operations *)
+| LT => "LT"
+| GT => "GT"
+| SLT => "SLT"
+| SGT => "SGT"
+| EQ => "EQ"
+| ISZERO => "ISZERO"
+| AND => "AND"
+| OR => "OR"
+| XOR => "XOR"
+| NOT => "NOT"
+| GETBYTE => "BYTE"
+    (* SHA3 *)
+| SHA3 => "SHA3"
+    (* Environmental Information *)
+| GETADDRESS => "ADDRESS"
+| BALANCE => "BALANCE"
+| ORIGIN => "ORIGIN"
+| CALLER => "CALLER"
+| CALLVALUE => "CALLVALUE"
+| CALLDATALOAD => "CALLDATASIZE"
+| CALLDATASIZE => "CALLDATASIZE"
+| CALLDATACOPY => "CALLDATACOPY"
+| CODESIZE => "CODESIZE"
+| CODECOPY => "CODECOPY"
+| GASPRICE => "GASPRICE"
+| EXTCODESIZE => "EXTCODESIZE"
+| EXTCODECOPY => "EXTCODECOPY"
+    (* Block Information *)
+| BLOCKHASH => "BLOCKHASH"
+| COINBASE => "COINBASE"
+| TIMESTAMP => "TIMESTAMP"
+| NUMBER => "NUMBER"
+| DIFFICULTY => "DIFFICULTY"
+| GASLIMIT => "GASLIMIT"
+    (* Stack, memory, storage and flow controls *)
+| POP => "POP"
+| MLOAD => "MLOAD"
+| MSTORE => "MSTORE"
+| MSTORE8 => "MSTORE8"
+| SLOAD => "SLOAD"
+| SSTORE => "SSTORE"
+| JUMP => "JUMP"
+| JUMPI => "JUMPI"
+| PC => "PC"
+| MSIZE => "MSIZE"
+| GAS => "GAS"
+| JUMPDEST => "JUMPDEST"
+    (* Push operations *)
+| PUSH1 => "PUSH1"
+| PUSH2 => "PUSH2"
+| PUSH3 => "PUSH3"
+| PUSH4 => "PUSH4"
+| PUSH5 => "PUSH5"
+| PUSH6 => "PUSH6"
+| PUSH7 => "PUSH7"
+| PUSH8 => "PUSH8"
+| PUSH9 => "PUSH9"
+| PUSH10 => "PUSH10"
+| PUSH11 => "PUSH11"
+| PUSH12 => "PUSH12"
+| PUSH13 => "PUSH13"
+| PUSH14 => "PUSH14"
+| PUSH15 => "PUSH15"
+| PUSH16 => "PUSH16"
+| PUSH17 => "PUSH17"
+| PUSH18 => "PUSH18"
+| PUSH19 => "PUSH19"
+| PUSH20 => "PUSH20"
+| PUSH21 => "PUSH21"
+| PUSH22 => "PUSH22"
+| PUSH23 => "PUSH23"
+| PUSH24 => "PUSH24"
+| PUSH25 => "PUSH25"
+| PUSH26 => "PUSH26"
+| PUSH27 => "PUSH27"
+| PUSH28 => "PUSH28"
+| PUSH29 => "PUSH29"
+| PUSH30 => "PUSH30"
+| PUSH31 => "PUSH31"
+| PUSH32 => "PUSH32"
+    (* Duplication operations *)
+| DUP1 => "DUP1"
+| DUP2 => "DUP2"
+| DUP3 => "DUP3"
+| DUP4 => "DUP4"
+| DUP5 => "DUP5"
+| DUP6 => "DUP6"
+| DUP7 => "DUP7" 
+| DUP8 => "DUP8"
+| DUP9 => "DUP9"
+| DUP10 => "DUP10"
+| DUP11 => "DUP11"
+| DUP12 => "DUP12"
+| DUP13 => "DUP13"
+| DUP14 => "DUP14"
+| DUP15 => "DUP15"
+| DUP16 => "DUP16"
+    (* Exchange Operations *)
+| SWAP1 => "SWAP1"
+| SWAP2 => "SWAP2"
+| SWAP3 => "SWAP3"
+| SWAP4 => "SWAP4"
+| SWAP5 => "SWAP5"
+| SWAP6 => "SWAP6"
+| SWAP7 => "SWAP7"
+| SWAP8 => "SWAP8"
+| SWAP9 => "SWAP9"
+| SWAP10 => "SWAP10"
+| SWAP11 => "SWAP11"
+| SWAP12 => "SWAP12"
+| SWAP13 => "SWAP13"
+| SWAP14 => "SWAP14"
+| SWAP15 => "SWAP15"
+| SWAP16 => "SWAP16"
+    (* Logging Operations *)
+| LOG0 => "LOG0"
+| LOG1 => "LOG1"
+| LOG2 => "LOG2"
+| LOG3 => "LOG3"
+| LOG4 => "LOG4"
+    (* System Operations *)
+| CREATE => "CREATE"
+| CALL => "CALL"
+| CALLCODE => "CALLCODE"
+| RETURN => "RETURN"
+| DELEGATECALL => "DELEGATECALL"
+| SUCIDE => "SUCIDE"
+| _ => "BADINSTR"
+   end)%string.
+
+
+(*--------------------------------------------------------------------
+ Unit test.
+ --------------------------------------------------------------------*)
 Compute (fromNatToInstr 243).
