src/program.v
@@ -2,46 +2,154 @@
  A program is represented as a list of BYTE.
  =====================================================================*)
 
-From mathcomp Require Import all_ssreflect.
-Require Import bitsops bitsrep instr.
+From Coq Require Import ZArith.ZArith Strings.String.
 
-Require Import List.
-Import ListNotations.
-Require Import listhelp.
+From mathcomp Require Import all_ssreflect.
+
+Require Import common_definitions bitsops bitsrep instr.
+
 
 (*=Program *)
-Definition Program := list BYTE.
+Definition Program := seq BYTE.
 (*=End *)
 
 (* BYTE to OpCode *)
 Definition BYTEToOpCode (b : BYTE) : Instr :=
-  let n := toNat (b : BYTE) in
-  fromNatToInstr n.
+  fromNatToInstr (toNat b).
 
 
 (* Get BYTE at postion [pc], counting from 0 *)
 Definition getCodeAt (pc : EVMWORD) (pro : Program) : option BYTE :=
-  let n := toNat pc in 
-  if (nth_ok n pro (#0 : BYTE)) then
-    Some (nth n pro (#0 : BYTE))
+  let n := toNat pc in
+  if (size pro) < (n + 1) then
+    None
   else
-    None.
-           
+    Some (nth (#0 : BYTE) pro n).
 
+           
+(* Add BYTE to a program *)
+Definition addBYTECode (b : BYTE) (pro : Program) : Program :=
+  rcons pro b.
+  
+(*---------------------------------------------------------------------
+ Program decoder: from Hex string to Program.
+ ---------------------------------------------------------------------*)
+Import Ascii.
+
+(* From BITS n to Program 
+   Return None (it is not well-formed) if the given sequence of bits 
+   is not divided into sequence of bytes
+ *)
+Fixpoint BITStoProgram {n} :=
+  match n return BITS n -> Program -> option Program with
+    | 0 => fun p pro => Some pro
+    | 1 => fun p pro => None
+    | 2 => fun p pro => None
+    | 3 => fun p pro => None
+    | 4 => fun p pro => None
+    | 5 => fun p pro => None
+    | 6 => fun p pro => None
+    | 7 => fun p pro => None
+    (* Extract 1 BYTE *)
+    | _ => fun p pro => let (hi, lo) := split2 _ 8 p in
+                           BITStoProgram hi (addBYTECode lo pro)
+  end.
+
+
+Definition HexToProgram s : option Program :=
+  match (BITStoProgram (fromHex s) nil) with
+    | None => None
+    | Some p => Some (rev p)
+  end.
+  
+
+(*---------------------------------------------------------------------
+ Check a program is well-formed.
+ A program is well-formed if
+ + It is a sequence of bytes
+ + For any byte that is not data of any PUSH instruction, it must be 
+   valid OpCode
+ + For any PUSH instruction, the number of bytes data is correct
+ ---------------------------------------------------------------------*)
+
+
+(*---------------------------------------------------------------------
+ Program to string.
+ ---------------------------------------------------------------------*)
+Fixpoint enumProgramToString (pro : Program) :=
+  (if pro is b::pro then
+    toHex b ++ " " ++ enumProgramToString pro
+  else "")%string.
+
+Definition programToString (pro : Program) :=
+  enumProgramToString pro.
+
+
+(*---------------------------------------------------------------------
+ EVM Assembly decoder. Notice that the program should be checked 
+ for well-formed one first. 
+ From Bytecode to OpCode.
+ ---------------------------------------------------------------------*)
+(* PUSH decoding. [pro] is the rest of program after PUSH *)
+Definition PUSHDecoding (n : nat) (pro : Program) : option (Program * Program) :=
+  if (size pro) < n then
+    None
+  else
+    Some ((take n pro), (drop n pro)).
+
+  
+Fixpoint enumProgramDecoding (pro : Program) :=
+  (if pro is b1::pro1 then
+     let i := BYTEToOpCode b1 in
+     match i with
+       | PUSH1 => match pro1 with
+                    | b2::pro2 => (instrToString i) ++ " " ++ (toHex b2) ++ " " ++ enumProgramDecoding pro2
+                    | nil => "Ill-formed program"
+                  end
+                    
+       | PUSH2 => match pro1 with
+                    | b2::b3::pro3 => (instrToString i) ++ " " ++ (toHex b2) ++ " " ++ (toHex b3) ++ " "  ++ enumProgramDecoding pro3
+                    | b2::nil => "Ill-formed program"
+                    | nil => "Ill-formed program"
+                  end
+       | PUSH3 => if (size pro1) < 3 then
+                    "Ill-formed program"
+                  else
+                    (instrToString i) ++ " " ++ (programToString (take 3 pro1)) ++ " " ++ enumProgramDecoding (drop 3 pro1)
+                                      
+       | _ => (instrToString i) ++ " " ++ enumProgramDecoding pro1
+     end
+   else
+     "")%string.
+
+
+                                     
 (*---------------------------------------------------------------------
  Unit test.
  ---------------------------------------------------------------------*)
-Example pro1 : Program := [(#96:BYTE); (#0:BYTE); (#53:BYTE); (#84:BYTE); (#25:BYTE); (#96:BYTE); (#9:BYTE); (#87:BYTE); (#0:BYTE); (#91:BYTE); (#96:BYTE); (#32:BYTE); (#53:BYTE);
-                (#96:BYTE); (#0:BYTE); (#53:BYTE); (#85:BYTE)].
+Example pro1 : Program := [::(#96:BYTE); (#0:BYTE); (#53:BYTE); (#84:BYTE);
+                           (#25:BYTE); (#96:BYTE); (#9:BYTE); (#87:BYTE);
+                           (#0:BYTE); (#91:BYTE); (#96:BYTE); (#32:BYTE);
+                           (#53:BYTE); (#96:BYTE); (#0:BYTE); (#53:BYTE);
+                           (#85:BYTE)].
 
 Compute (
     let oInstr := getCodeAt (#2:EVMWORD) pro1 in
     match oInstr with
-      | Some b => BYTEToOpCode b
-      | None => BADINSTR
+      | Some b => instrToString (BYTEToOpCode b)
+      | None => "Out-Of-Bound"%string 
     end
   ).
 
+Example HexProgram := "6000355419600957005B60203560003555"%string.
+
+Compute (
+    let pro := HexToProgram HexProgram in
+    match pro with
+      | None => ""%string
+      | Some p => programToString p
+    end
+      ).
 
 
 
